sample send API

src/tls/HandshakeLogLow.fsti
@@ -1,5 +1,6 @@
 module HandshakeLogLow
 
+open FStar.Bytes
 open FStar.Integers
 open FStar.HyperStack.ST
 
@@ -84,6 +85,10 @@ let valid_transcript (msgs:list msg) =
 
 type hs_transcript : Type0 = msgs:list msg{valid_transcript msgs}
 
+/// Bytes from the transcript
+
+val transcript_bytes: hs_transcript -> GTot bytes
+
 
 /// HSL main API
 
@@ -102,37 +107,45 @@ val hsl_invariant : HS.mem -> hsl_state -> Type0
 
 /// Length of the input buffer that HSL reads from
 
-val hsl_input_buf_len : hsl_state -> uint_32
+val hsl_input_buf_len : hsl_state -> GTot uint_32
 
 
 /// Input buffer itself
 
-val hsl_input_buf : st:hsl_state -> lbuffer8 (hsl_input_buf_len st)
+val hsl_input_buf : st:hsl_state -> GTot (lbuffer8 (hsl_input_buf_len st))
 
 
 /// Index of the input buffer where HSL is at
+/// Client (Record) should only add to the buffer at and after this index
 
-val hsl_input_index : HS.mem -> st:hsl_state -> i:uint_32{i <= hsl_input_buf_len st}
+val hsl_input_index : HS.mem -> st:hsl_state -> GTot (i:uint_32{i <= hsl_input_buf_len st})
 
 
-/// Length of the output buffer that HSL writes to
+/// Length of the output buffer, Handshake writes to it
 
-val hsl_output_buf_len : hsl_state -> uint_32
+val hsl_output_buf_len : hsl_state -> GTot uint_32
 
 
 /// Output buffer itself
 
-val hsl_output_buf : st:hsl_state -> lbuffer8 (hsl_output_buf_len st)
+val hsl_output_buf : st:hsl_state -> GTot (lbuffer8 (hsl_output_buf_len st))
+
+
+/// Index of the output buffer where HSL is at
+/// Client (Handshake) should only add to the buffer at and after this index
+
+val hsl_output_index : HS.mem -> st:hsl_state -> GTot (i:uint_32{i <= hsl_output_buf_len st})
 
 
 /// HSL footprint
+/// Local footprint is abstract and is allocated in the region provided at the creation time
 
 val hsl_local_footprint : hsl_state -> B.loc
 
 let hsl_footprint (h:HS.mem) (st:hsl_state) : GTot B.loc =
   let open B in
   loc_union (hsl_local_footprint st)  //local footprint
-            (loc_union (loc_buffer (hsl_output_buf st))  //output buffer
+            (loc_union (loc_buffer (gsub (hsl_output_buf st) 0ul (hsl_output_index h st)))  //output buffer upto index
                        (loc_buffer (gsub (hsl_input_buf st) 0ul (hsl_input_index h st))))  //input buffer upto index
 
 
@@ -158,7 +171,8 @@ val elim_hsl_invariant (st:hsl_state) (h:HS.mem)
   : Lemma (requires (hsl_invariant h st))
           (ensures  (B.live h (hsl_input_buf st) /\ B.live h (hsl_output_buf st) /\
 	             B.loc_pairwise_disjoint [hsl_local_footprint st; B.loc_buffer (hsl_input_buf st);
-		                              B.loc_buffer (hsl_output_buf st)]))
+		                              B.loc_buffer (hsl_output_buf st)] /\
+	             valid_transcript (transcript h st)))
 	  [SMTPat (hsl_invariant h st)]
 
 /// Invariant framing
@@ -180,6 +194,7 @@ unfold private let create_post (r:Mem.rgn)
     hsl_input_buf_len st == input_len /\ hsl_input_buf st == input_buf /\
     hsl_output_buf_len st == output_len /\ hsl_output_buf st == output_buf /\  //I/O bufs are as given
     hsl_input_index h1 st == 0ul /\  //input index is 0
+    hsl_output_index h1 st == 0ul /\  //output index is 0
     B.fresh_loc (hsl_local_footprint st) h0 h1 /\  //local footprint is fresh
     B.loc_includes (B.loc_regions true (Set.singleton r)) (hsl_local_footprint st) /\  //TODO: local footprint is in r only
     hsl_invariant h1 st /\  //invariant holds
@@ -191,7 +206,9 @@ unfold private let create_post (r:Mem.rgn)
 val create (r:Mem.rgn) (pv:option C.protocolVersion)
            (input_len:uint_32) (input_buf:lbuffer8 input_len)
 	   (output_len:uint_32) (output_buf:lbuffer8 output_len)
-  : ST hsl_state (requires (fun _ -> B.loc_disjoint (B.loc_buffer input_buf) (B.loc_buffer output_buf)))
+  : ST hsl_state (requires (fun h0 -> 
+                            B.live h0 input_buf /\ B.live h0 output_buf /\
+                            B.loc_disjoint (B.loc_buffer input_buf) (B.loc_buffer output_buf)))  //disjoint I/O buffers
                  (ensures  (create_post r input_len input_buf output_len output_buf))
 
 
@@ -201,12 +218,20 @@ unfold private let set_params_post (st:hsl_state) (a:Hashing.alg)
   : HS.mem -> unit -> HS.mem -> Type0
 
   = fun h0 _ h1 ->
-    B.modifies (hsl_local_footprint st) h0 h1 /\
-    transcript h1 st == transcript h0 st /\
-    writing h1 st == writing h0 st /\
-    hsl_input_index h1 st == hsl_input_index h0 st /\
-    hash_alg h1 st == Some a /\
-    hsl_invariant h1 st  //NB: we are not saying hsl_footprint is same explicitly, it is derivable though
+    B.modifies (hsl_local_footprint st) h0 h1 /\  //modifies only local footprint
+    transcript h1 st == transcript h0 st /\  //transcript remains same
+    writing h1 st == writing h0 st /\  //writing capability remains same
+    hsl_input_index h1 st == hsl_input_index h0 st /\  //input index remains same
+    hsl_output_index h1 st == hsl_output_index h0 st /\  //output index remains same
+    hash_alg h1 st == Some a /\  //hash algorithm is set
+    hsl_invariant h1 st  //invariant holds
+                         //NB: we are not saying hsl_footprint is same explicitly, it is derivable though, as shown below
+
+private let footprint_remains_same_across_set_params
+  (st:hsl_state) (a:Hashing.alg) (h0 h1:HS.mem)
+  : Lemma (requires (set_params_post st a h0 () h1))
+          (ensures  (hsl_footprint h0 st == hsl_footprint h1 st))
+  = ()
 
 val set_params (st:hsl_state) (_:C.protocolVersion) (a:Hashing.alg) (_:option CipherSuite.kexAlg)
                (_:option CommonDH.group)
@@ -224,15 +249,14 @@ val tags (a:Hash.alg) (prior:list msg) (ms:list msg) (hs:list HashSpec.anyTag) :
 val hs_transcript_parser : LP.parser (LP.strong_parser_kind 8 8 ({ LP.parser_kind_metadata_total = true })) hs_transcript
 
 (* msgs is parsing of the input sub-buffer between p0 and p1 *)
-unfold private let parsing_of (msgs:hs_transcript) (st:hsl_state)
-                              (p0:uint_32) (p1:uint_32{p0 <= p1 /\ p1 <= hsl_input_buf_len st})
-			      (h:HS.mem)
+unfold private let transcript_parsing_of (msgs:hs_transcript) (st:hsl_state)
+                                         (p0:uint_32) (p1:uint_32{p0 <= p1 /\ p1 <= hsl_input_buf_len st})
+			                 (h:HS.mem)
   = let delta = p1 - p0 in
     let sub = B.gsub (hsl_input_buf st) p0 delta in
     match LP.parse hs_transcript_parser (B.as_seq h sub) with
     | None -> False
-    | Some (parse, consumed) ->
-      parse == msgs /\ consumed == v delta (* unsure about the latter part *)
+    | Some (parse, consumed) -> parse == msgs /\ consumed == v delta
 
 unfold private let receive_post (st:hsl_state) (p:uint_32)
   : HS.mem -> (TLSError.result (option (G.erased hs_transcript &
@@ -246,6 +270,7 @@ unfold private let receive_post (st:hsl_state) (p:uint_32)
     B.modifies (hsl_local_footprint st) h0 h1 /\  //only local footprint is modified
     hash_alg h1 st == oa /\  //hash alg remains same
     hsl_invariant h1 st /\  //invariant holds
+    hsl_output_index h1 st == hsl_output_index h0 st /\  //output index remains same
     hsl_input_index h1 st == p /\  //input index is advanced to p
     (match r with
      | Error _ -> True  //underspecified
@@ -256,7 +281,7 @@ unfold private let receive_post (st:hsl_state) (p:uint_32)
        writing h1 st /\  //Handshake can now write
        p <= hsl_input_buf_len st /\
        p0 <= p1 /\ p1 <= p /\  //returned indices are valid in the input buffer
-       parsing_of ms st p0 p1 h1 /\  //ms is a valid parsing of input buffer contents between p0 and p1
+       transcript_parsing_of ms st p0 p1 h1 /\  //ms is a valid parsing of input buffer contents between p0 and p1
        (match oa with
         | Some a -> tags a t0 ms hs  //hashed properly
         | None -> hs == []))
@@ -270,3 +295,62 @@ val receive (st:hsl_state) (p:uint_32)
                   hsl_input_index h0 st <= p /\  //TODO: should have written >= 0 bytes (> 0?)
 		  p <= hsl_input_buf_len st))  //p should be in the input buffer range
        (ensures  (receive_post st p))
+
+
+/// TODO: receive_CCS
+
+
+/// Send API
+
+/// TODO: should come from QD
+
+val msg_parser : LP.parser (LP.strong_parser_kind 8 8 ({ LP.parser_kind_metadata_total = true })) msg
+
+unfold private let msg_parsing_of (m:msg) (st:hsl_state)
+                                  (p0:uint_32) (p1:uint_32{p0 <= p1 /\ p1 <= hsl_output_buf_len st})
+			          (h:HS.mem)
+  = let delta = p1 - p0 in
+    let sub = B.gsub (hsl_output_buf st) p0 delta in
+    match LP.parse msg_parser (B.as_seq h sub) with
+    | None -> False
+    | Some (parse, consumed) -> parse == m /\ consumed == v delta
+
+unfold private let send_pre (st:hsl_state) (p:uint_32) (m:G.erased msg)
+  : HS.mem -> Type0
+  = fun h0 ->
+    let open HandshakeMessages in
+    hsl_invariant h0 st /\  //invariant holds
+    hsl_output_index h0 st <= p /\ p <= hsl_output_buf_len st /\  //p is in range of output buffer
+    msg_parsing_of (G.reveal m) st (hsl_output_index h0 st) p h0 /\  //m is a valid parsing of sub-buffer between p0 and p1
+    writing h0 st /\  //Handshake is allowed to write
+    valid_transcript (transcript h0 st @ [G.reveal m]) /\  //valid transcript
+    (match G.reveal m with  //copied from HandshakeLog as is
+     | HelloRetryRequest req -> Some? (C.cipherSuite_of_name req.hrr_cipher_suite)
+     | _ -> True)
+
+unfold private let send_post (st:hsl_state) (p:uint_32) (m:G.erased msg)
+  : HS.mem -> unit -> HS.mem -> Type0
+  = fun h0 _ h1 ->
+    B.modifies (hsl_local_footprint st) h0 h1 /\  //only local footprint is modified
+    writing h1 st /\  //writing capability remains
+    hash_alg h1 st == hash_alg h0 st /\  //hash algorithm is same as before
+    transcript h1 st == transcript h0 st @ [G.reveal m] /\  //transcript includes m
+    hsl_invariant h1 st /\  //invariant hold
+    hsl_input_index h1 st == hsl_input_index h0 st /\  //input buffer index remains same
+    hsl_output_index h1 st == p  //output buffer index is advanced to p
+
+val send (st:hsl_state) (p:uint_32) (m:G.erased msg)
+  : ST unit (requires (send_pre st p m))
+            (ensures  (send_post st p m))
+		       
+/// hash_tag API
+
+/// TODO: the postcondition fails to typecheck
+
+#push-options "--admit_smt_queries true"
+val hash_tag (a:Hash.alg) (st:hsl_state)
+  : ST (Hash.tag a) (requires (fun h0 -> hsl_invariant h0 st))
+                    (ensures  (fun h0 r h1 ->
+		               let bs = transcript_bytes (transcript h1 st) in
+			       h0 == h1 /\ Hashing.CRF.hashed a bs /\ r == Hash.h a bs))
+#pop-options
